\documentclass{article}
\usepackage[left=2cm,right=2cm,top=3cm,bottom=3cm]{geometry}
\usepackage{mathtools}
\usepackage{amsmath}
\usepackage{bbold}
\begin{document}
Let $L(f) = \sum_{n\in \mathbb{Z}} f(n)$. First, show $L$ is linear:
\begin{align*}
L(f + g) &= \sum_{n \in \mathbb{Z}} (f + g)(n)\\
&= \sum_{n \in \mathbb{Z}} f(n) + \sum_{n \in \mathbb{Z}} g(n)\\
&= L(f) + L(g)
&\textit{So, additive. Now show homogenous:}\\
L(\lambda f) &= \sum_{n \in \mathbb{Z}} \lambda f(n)\\
&= \lambda L(f)
\end{align*}
So $L$ is a linear map from $V \rightarrow \mathbb{C}$. Now suppose, by contradiction that $\exists v \in V: L(w) = \langle w, v \rangle \forall w$. Then, have $L(w) = \sum_{n} w(n) \overline{v(n)}$. Now, there are finitely many $n: \overline{v(n)} \neq 0$. Let $s = \{n\in \mathbb{Z}: \overline{V(n)}\} = \neq 0$. Let $M = \mathbb{Z}/s$. Define take some finite subset of $M$ with all positive entries, call it $m$. Define 
\[ g:\mathbb{Z} \rightarrow C: g(x) = 
\begin{cases} 
 x \in m & x\\ 
 x \notin m & 0\\
 \end{cases} \]
Then g is nonzero at only the cardinality of $m$ points, which is finite, so $g \in V$, but $L(g) = \sum (m_{i} \in m)$, but $\langle g, v \rangle = 0$, since $v$ is 0 everywhere $g$ is nonzero, contradicting our assumption that $v$ worked for all $f \in V$, as desired.
\end{document}
